Rewrote compute in a new file, do_computation. Fixed this so it can compute on more constants and actually do some useful things (the old version of compute had a bug where it could only do computations on trivial const functions that were data constructors with no arguments).
Reordered functions in functions.v in order to sort functions that
can compute into consts from those that can't.

reify/functions.v
@@ -196,11 +196,11 @@ Expr.Sig all_types nil Z_tv Int.max_unsigned.
 Import ListNotations.
 
 Definition functions :=
-[ tc_environ_signature
+[ two_power_nat_signature 
 ; O_signature
 ; force_ptr_signature
 ; app_val_signature
-; eval_id_signature
+; int_max_unsigned_signature 
 ; and_signature
 ; align_signature
 ; cons_val_signature 
@@ -242,16 +242,15 @@ Definition functions :=
 ; int_repr_signature
 ; int_signed_signature
 ; int_unsigned_signature
-; two_power_nat_signature
-; int_max_unsigned_signature
+; tc_environ_signature
+; eval_id_signature
 ].
 
-
-Definition tc_environ_f := 0%nat.
+Definition two_power_nat_f := 0%nat.
 Definition O_f := 1%nat.
 Definition force_ptr_f := 2%nat.
 Definition app_val_f := 3%nat.
-Definition eval_id_f := 4%nat.
+Definition int_max_unsigned_f := 4%nat.
 Definition and_f := 5%nat.
 Definition align_f := 6%nat.
 Definition cons_val_f := 7%nat.
@@ -293,10 +292,11 @@ Definition int_cmpu_f := 42%nat.
 Definition int_repr_f := 43%nat.
 Definition int_signed_f := 44%nat.
 Definition int_unsigned_f := 45%nat.
-Definition two_power_nat_f := 46%nat.
-Definition int_max_unsigned_f := 47%nat.
+(* Past this point are functions that should not compute into Consts *)
+Definition tc_environ_f := 46%nat.
+Definition eval_id_f := 47%nat.
 
-Check field_at.
+Definition end_const_index := 46%nat.
 
 
 (*Separation Logic predicates *)
