reify/do_computation.v
@@ -1,0 +1,95 @@
+(* compute.v - Mario Alvarez - January 2014
+ * Implementation of "compute" solver plugin for MirrorShard *)
+
+(* Need all of these? *)
+Require Import floyd.proofauto.
+Require Import types.
+Require Import functions.
+Require Import progs.reverse.
+Require Import progs.list_dt.
+Require Import sep.
+Require Import Expr.
+
+Module do_computation (uk : unknown_types).
+Module our_funcs := funcs uk.
+Import our_funcs.
+Import all_types.
+
+(* Cleaner syntax for Nat pattern-matches and function lists *)
+Local Open Scope nat.
+Import List.
+Import ListNotations.
+
+(* Listing of which functions compute directly into consts (taking no arguments)
+ * and which do not. *)
+(*
+Definition is_const_base (f : func) :=
+  match f with
+    | 1  (* O_f *)
+    | 20 (* Z0_f *)
+    | 23 (* xH_f *)
+    | 35 (* Ceq_f *)
+    | 36 (* Cne_f *)
+    | 37 (* Clt_f *)
+    | 38 (* Cle_f *)
+    | 39 (* Cgt_f *)
+    | 40 (* Cge_f *)
+    | 47 (* int_max_unsigned *)
+      => true
+
+    | _ => false
+  end.            
+*)
+
+Definition is_const_base (f : func) :=
+NPeano.ltb f end_const_index.
+
+(* Decide if an expression can compute directly into a Const
+ * (by converting the pre-defined functions we have defined
+ * as convertible into consts) *)
+Fixpoint is_const (e : expr all_types) :=
+  let is_const_l (es : list (expr all_types)) : bool :=
+      fold_right andb true (map is_const es)
+  in
+  match e with
+      (* it and its arguments must be const *)
+    | Func f es => andb (is_const_base f) (is_const_l es)
+    | Const _ _ => true
+    | _ => false
+  end.             
+
+(* Simplify an expression, if we can.
+ * Expects that a user-supplied Ltac will have already converted
+ * user-defined functions into Consts, as appropriate *)
+Definition do_computation (user_functions : list (signature all_types)) (e : expr all_types) (t : tvar) : 
+option (tvarD all_types t) := (*expr all_types :=*)
+if is_const e then
+  match (@exprD all_types (functions ++ user_functions) nil nil e t) with
+    | Some v => Some v
+    | None => None (** should be dead code if e is well typed **)
+  end
+else
+  None.
+
+
+Lemma do_computation_correct : forall (user_functions : list (signature all_types)) (e : expr all_types) (t : tvar) (v : tvarD all_types t),
+do_computation user_functions e t = Some v ->
+forall (vars uvars : env all_types),
+exprD (functions ++ user_functions) uvars vars e t = Some v.
+Proof.
+  intros.
+  unfold do_computation in *.
+  destruct (is_const e); try congruence.
+  remember (exprD (functions ++ user_functions) [] [] e t) as exprDf.
+  destruct exprDf.
+  - inversion H; subst.
+    symmetry in HeqexprDf.
+    eapply exprD_weaken in HeqexprDf.
+    eassumption.
+  - inversion H.
+Qed.
+
+(* Some fun little examples *)
+Eval vm_compute in (do_computation nil (Func 13 [(Func 1 [])]) (tvType 11)).
+
+End do_computation.
